Capless/Subst/Capture/Typing.lean
@@ -131,6 +131,16 @@ theorem Typed.csubst
          , <- CaptureSet.weaken_crename
          , <- CaptureSet.cweaken_crename ] at ih
       aesop
+    case intercept ih ih2 =>
+      simp [Term.crename]
+      apply intercept
+      have ih := ih $ (σ.text.ext _).ext _
+      simp [TBinding.crename, EType.crename, CType.crename, SType.crename] at ih ih2
+      simp [← SType.weaken_crename, ← SType.tweaken_crename, ← CaptureSet.weaken_crename, CaptureSet.proj_crename] at ih ih2
+      apply ih
+      apply! ih2
+
+
 
 theorem Typed.copen
   (h : Typed (Γ,c<:CBound.upper {c=c|.top}) t E Ct) :
